\section{Introduction}
$\emph{FV}(\Gamma)=\bigcup\{\emph{FV}(t)\mid (x:t)\in \Gamma\}$\\
$\lambda2$ deduction Rules
\begin{mdframed}
\begingroup
\addtolength{\jot}{0.3cm}
\begin{align*}
&(\text{Axiom}) &&\Gamma,x:t\vdash x:t\\
&(\lambda\text{-Introduction}) &&\frac{\Gamma,x:t_1\vdash e:t_2}{\Gamma\vdash \lambda x.e:t_1\to t_2}\\
&(\lambda\text{-Elimination}) &&\frac{\Gamma\vdash e_1:t_1\to t_2 \hspace{0.4cm}\Gamma\vdash e_2:t_1}{\Gamma\vdash e_1e_2:t_2}\\
&(\forall\text{-Introduction}) &&\frac{\Gamma\vdash e:t}{\Gamma\vdash \Lambda\alpha.e:\forall\alpha.t} &&\alpha\notin\FV(\Gamma) \\
&(\forall\text{-Elimination}) &&\frac{\Gamma\vdash e:\forall\alpha.t }{\Gamma\vdash et':t\left[ \alpha:=t'\right] }
\end{align*}
\endgroup
\end{mdframed}
